core/Implies.v
@@ -1,0 +1,155 @@
+Require Import Coq.ZArith.ZArith.
+Require Import Poulet4.Typed.
+Require Import Poulet4.Syntax.
+Require Import Poulet4.Value.
+Require Import Poulet4.Semantics.
+Require Import ProD3.core.Coqlib.
+Require Import ProD3.core.SvalRefine.
+Require Import ProD3.core.AssertionLang.
+Require Import ProD3.core.AssertionNotations.
+Require Import ProD3.core.Hoare.
+Require Import Poulet4.SyntaxUtil.
+Require Import Hammer.Plugin.Hammer.
+
+Section Implies.
+
+Context {tags_t: Type} {tags_t_inhabitant : Inhabitant tags_t}.
+Notation Val := (@ValueBase bool).
+Notation Sval := (@ValueBase (option bool)).
+Notation Lval := (@ValueLvalue tags_t).
+
+Notation ident := (String.string).
+Notation path := (list ident).
+Notation Expression := (@Expression tags_t).
+
+Context {target : @Target tags_t Expression}.
+
+Definition mem_simplify_aux (a : mem_assertion) '((p, sv) : path * Sval) : option (Sval * Sval) :=
+  match AList.get a p with
+  | Some sv' => Some (sv, sv')
+  | None => None
+  end.
+
+Lemma mem_simplify_aux_sound : forall a psv svp,
+  mem_simplify_aux a psv = Some svp ->
+  uncurry sval_refine svp ->
+  forall m, mem_denote a m -> mem_satisfies_unit m psv.
+Proof.
+  intros.
+  destruct psv as [p sv].
+  unfold mem_simplify_aux in *.
+  destruct (AList.get a p) eqn:H_get; inv H.
+  eapply mem_denote_get in H_get; eauto.
+  unfold mem_satisfies_unit in *.
+  destruct (PathMap.get p m); only 2 : inv H_get.
+  eapply sval_refine_trans; eauto.
+Qed.
+
+Definition mem_implies_simplify (a a' : mem_assertion) : option (list (Sval * Sval)) :=
+  lift_option (map (mem_simplify_aux a) a').
+
+Lemma fold_right_and_True : forall l,
+  fold_right and True l <-> Forall id l.
+Proof.
+  intros; induction l; only 2 : destruct IHl; split; intros.
+  - constructor.
+  - constructor.
+  - constructor; sfirstorder.
+  - inv H1; sfirstorder.
+Qed.
+
+Lemma mem_implies_simplify_sound : forall a a' svps,
+  mem_implies_simplify a a' = Some svps ->
+  Forall (uncurry sval_refine) svps ->
+  forall m, mem_denote a m -> mem_denote a' m.
+Proof.
+  intros.
+  unfold mem_implies_simplify in *.
+  apply lift_option_inv in H.
+  unfold mem_denote, mem_satisfies.
+  rewrite fold_right_and_True in *.
+  list_simplify.
+  apply mem_simplify_aux_sound with a (Znth i svps).
+  - list_simplify.
+    (* list_solve cannot perform this simplification because the implicit type mem_unit and (path * Sval)
+      are not converted automatically. *)
+    rewrite Znth_map in H12 by auto. list_solve.
+  - list_solve.
+  - auto.
+Qed.
+
+Definition ext_simplify_aux (a : ext_assertion) '((p, eo) : path * extern_object) : option (extern_object * extern_object) :=
+  match AList.get a p with
+  | Some eo' => Some (eo, eo')
+  | None => None
+  end.
+
+Lemma ext_simplify_aux_sound : forall a peo eop,
+  ext_simplify_aux a peo = Some eop ->
+  uncurry eq eop ->
+  forall es, ext_denote a es -> ext_satisfies_unit es peo.
+Proof.
+  intros.
+  destruct peo as [p eo].
+  unfold ext_simplify_aux in *.
+  destruct (AList.get a p) eqn:H_get; inv H.
+  eapply ext_denote_get in H_get; eauto.
+  inv H0.
+  auto.
+Qed.
+
+Definition ext_implies_simplify (a a' : ext_assertion) : option (list (extern_object * extern_object)) :=
+  lift_option (map (ext_simplify_aux a) a').
+
+Lemma ext_implies_simplify_sound : forall a a' eops,
+  ext_implies_simplify a a' = Some eops ->
+  Forall (uncurry eq) eops ->
+  forall m, ext_denote a m -> ext_denote a' m.
+Proof.
+  intros.
+  unfold ext_implies_simplify in *.
+  apply lift_option_inv in H.
+  unfold ext_denote, ext_satisfies.
+  rewrite fold_right_and_True in *.
+  (* Cannot use list_solve because there's no Inhabitant for extern_object. *)
+  generalize dependent a'.
+  induction H0; intros.
+  - destruct a'; inv H.
+    constructor.
+  - destruct a'; inv H2.
+    constructor.
+    + eapply ext_simplify_aux_sound; eauto.
+    + eauto.
+Qed.
+
+Lemma implies_simplify : forall pre_mem pre_ext post_mem post_ext svps eops,
+  mem_implies_simplify pre_mem post_mem = Some svps ->
+  Forall (uncurry sval_refine) svps ->
+  ext_implies_simplify pre_ext post_ext = Some eops ->
+  Forall (uncurry eq) eops ->
+  implies (MEM pre_mem (EXT pre_ext)) (MEM post_mem (EXT post_ext)).
+Proof.
+  unfold implies; intros.
+  destruct st as [m es].
+  destruct H3; split.
+  - eapply mem_implies_simplify_sound; eauto.
+  - eapply ext_implies_simplify_sound; eauto.
+Qed.
+
+Lemma implies_simplify_ret : forall pre_mem pre_ext post_ret post_mem post_ext retv svps eops,
+  (forall sv' : Sval, val_to_sval retv sv' -> ret_denote post_ret sv') ->
+  mem_implies_simplify pre_mem post_mem = Some svps ->
+  Forall (uncurry sval_refine) svps ->
+  ext_implies_simplify pre_ext post_ext = Some eops ->
+  Forall (uncurry eq) eops ->
+  implies (MEM pre_mem (EXT pre_ext)) (RET post_ret (MEM post_mem (EXT post_ext)) retv).
+Proof.
+  unfold implies; intros.
+  destruct st as [m es].
+  destruct H4; split; only 2 : split.
+  - eauto.
+  - eapply mem_implies_simplify_sound; eauto.
+  - eapply ext_implies_simplify_sound; eauto.
+Qed.
+
+End Implies.
