examples/bloomfilter/verif.v
@@ -70,6 +70,12 @@ Proof.
   intros.
   start_function.
   forward.
+  forward.
+  entailer.
+  - admit.
+  - constructor. { apply SvalRefine.sval_refine_refl. }
+    constructor.
+  - constructor.
 Admitted.
 
 Lemma MyIngress_do_forward_spec : forall p (port : Z) (standard_metadata : Sval),
